Specify and prove helper for `allowance`
Based very closely on and imports: `Generated/erc20shim/ERC20Shim/mapping_index_access_mapping_address_mapping_address_uint256_of_address_user.lean`

Generated/erc20shim/ERC20Shim/mapping_index_access_mapping_address_mapping_address_uint256_of_address_user.lean
@@ -2,7 +2,7 @@ import Clear.ReasoningPrinciple
 
 
 import Generated.erc20shim.ERC20Shim.mapping_index_access_mapping_address_mapping_address_uint256_of_address_gen
-
+import Generated.erc20shim.ERC20Shim.mapping_index_access_mapping_address_uint256_of_address_user
 
 namespace Generated.erc20shim.ERC20Shim
 
@@ -10,13 +10,46 @@ section
 
 open Clear EVMState Ast Expr Stmt FunctionDefinition State Interpreter ExecLemmas OutOfFuelLemmas Abstraction YulNotation PrimOps ReasoningPrinciple Utilities 
 
-def A_mapping_index_access_mapping_address_mapping_address_uint256_of_address (dataSlot : Identifier) (slot key : Literal) (s₀ s₉ : State) : Prop := sorry
+def A_mapping_index_access_mapping_address_mapping_address_uint256_of_address (dataSlot : Identifier) (slot key : Literal) (s₀ s₉ : State) : Prop :=
+  A_mapping_index_access_mapping_address_uint256_of_address dataSlot slot key s₀ s₉
 
 lemma mapping_index_access_mapping_address_mapping_address_uint256_of_address_abs_of_concrete {s₀ s₉ : State} {dataSlot slot key} :
   Spec (mapping_index_access_mapping_address_mapping_address_uint256_of_address_concrete_of_code.1 dataSlot slot key) s₀ s₉ →
   Spec (A_mapping_index_access_mapping_address_mapping_address_uint256_of_address dataSlot slot key) s₀ s₉ := by
-  unfold mapping_index_access_mapping_address_mapping_address_uint256_of_address_concrete_of_code A_mapping_index_access_mapping_address_mapping_address_uint256_of_address
-  sorry
+  unfold mapping_index_access_mapping_address_mapping_address_uint256_of_address_concrete_of_code A_mapping_index_access_mapping_address_mapping_address_uint256_of_address A_mapping_index_access_mapping_address_uint256_of_address
+  rcases s₀ with ⟨evm, varstore⟩ | _ | _ <;> [simp only; aesop_spec; aesop_spec]
+  apply spec_eq
+  intro hasFuel
+  clr_funargs
+
+  rw [ EVMSub', EVMShl', EVMAddrSize' ]; simp
+  rw [ Address.and_size_eq_ofUInt256 ]
+  rw [ multifill_cons, multifill_nil ]
+  simp
+
+  clr_varstore
+
+  generalize account_def : Address.ofUInt256 key = account
+  intro prog erc20 account_mem_balances address hasAddress
+
+  generalize prep_def : (mstore evm 0 ↑↑account).mstore 32 slot = state_prep
+  unfold keccak256 at prog
+  rw [ interval'_eq_interval 2 two_ne_zero (by norm_cast)
+     , mstore_mstore_of_ne, interval_of_mstore_eq_val_cons
+     , mstore_mstore_of_ne, zero_add, interval_of_mstore_eq_val_cons
+     , interval_of_0_eq_nil
+     ] at prog
+  unfold_let at prog
+  rw [ mstore_preserves_keccak_map, mstore_preserves_keccak_map
+     , hasAddress
+     ] at prog
+  simp at prog
+  unfold setEvm State.insert State.lookup! at prog
+  simp at prog
+
+  rw [← prog]
+  unfold State.lookup!
+  simp
 
 end
 
